theories/array.v
@@ -1,11 +1,14 @@
 (** a naive functional representation of an array *)
 (* (C) J. Pichon - see LICENSE.txt *)
 
+From mathcomp Require Import ssreflect ssrbool eqtype.
+
 (* this works well when there are few updates *)
 Module Type Index_Sig.
 Parameter Index : Type.
 Parameter index_eqb : Index -> Index -> bool.
 Parameter Value : Type.
+Axiom index_eqb_eqP : Equality.axiom index_eqb.
 End Index_Sig.
 
 Module Make (X : Index_Sig).
@@ -28,6 +31,26 @@ Fixpoint get (arr : array) (idx : Index) : Value :=
 
 Fixpoint set (arr : array) (idx : Index) (a : Value) : array :=
   A_update idx a arr.
+
+Lemma get_set : forall i v arr,
+  get (set arr i v) i = v.
+Proof.
+move => i v.
+rewrite /get /set.
+case; rewrite (introT (index_eqb_eqP i i) (Logic.eq_refl i)); reflexivity.
+Qed.
+
+Lemma get_skip : forall i i' v arr,
+  index_eqb i i' = false ->
+  get (set arr i' v) i = get arr i.
+Proof.
+move => i i' v arr His.
+case: arr.
+{ move => v_init.
+  by rewrite /get /set His. }
+{ move => i'' v'' a.
+  by rewrite /= His. }
+Qed.
 
 End Make.
 
